theories/iris_extra.v
@@ -1,0 +1,24 @@
+From Coq Require Import ssreflect.
+From stdpp Require Import gmap.
+From transfinite.base_logic.lib Require Import own.
+From iris.algebra Require Import auth excl excl_auth gmap.
+From iris.proofmode Require Import tactics.
+From iris.prelude Require Import options.
+
+Section Extra.
+Context `{SI: indexT}.
+Context {Σ : gFunctors}.
+
+Lemma big_sepM_of_pairs {A B} `{Countable A, Countable (A * B)} (m: gmap A B) (Φ : A → B → iProp Σ):
+  ([∗ set] p ∈ map_to_set pair m, Φ p.1 p.2) -∗
+  ([∗ map] k↦v ∈ m, Φ k v).
+Proof.
+  induction m using map_ind; first by eauto.
+  iIntros "Hs". iApply big_sepM_insert; first done.
+  rewrite map_to_set_insert_L//.
+  iDestruct (big_sepS_insert with "Hs") as "($&Hs)".
+  { intros ?%elem_of_map_to_set_pair. congruence. }
+  iApply (IHm with "Hs").
+Qed.
+
+End Extra.
